ulib/experimental/Steel.C.Reference.fsti
@@ -1,0 +1,266 @@
+module Steel.C.Reference
+open Steel.C.Model.PCM
+open Steel.C.Model.Ref
+open Steel.Effect
+open Steel.Effect.Atomic
+
+val ptr (view_t: Type u#0) (#b: Type u#b) (q: pcm b)
+: Type u#b
+
+val null (view_t: Type u#0) (#b: Type u#b) (p: pcm b) : Tot (ptr view_t p)
+
+val ptr_is_null (#view_t: Type u#0) (#b: Type u#b) (#q: pcm b) (p: ptr view_t q) : Ghost bool
+  (requires True)
+  (ensures (fun y -> y == true <==> p == null view_t q))
+
+// [@@__reduce__]
+inline_for_extraction
+let ref (view_t: Type u#0) (#b: Type u#b) (q: pcm b)
+: Tot (Type u#b)
+=
+  (x: ptr view_t q { ptr_is_null x == false })
+
+val pts_to_view_hp
+  (#view_t: Type u#0)
+  (#view_t': Type u#0)
+  (#b: Type u#b) (#p: pcm b)
+  (r: ref view_t p) (view: sel_view p view_t' false)
+: Tot (Steel.Memory.slprop u#1)
+
+val pts_to_view_sel
+  (#view_t: Type u#0)
+  (#view_t': Type u#0)
+  (#b: Type u#b) (#p: pcm b)
+  (r: ref view_t p) (view: sel_view p view_t' false)
+: Tot (selector view_t' (pts_to_view_hp r view))
+
+[@@__steel_reduce__]
+let pts_to_view
+  (#view_t: Type u#0)
+  (#view_t': Type u#0)
+  (#b: Type u#b) (#p: pcm b)
+  (r: ref view_t p) (view: sel_view p view_t' false)
+: vprop
+= VUnit ({
+    hp = pts_to_view_hp r view;
+    t = _;
+    sel = pts_to_view_sel r view;
+  })
+
+val ref_read
+  (#b: Type u#b)
+  (#view_t: Type u#0)
+  (#p: pcm b)
+  (#vw: sel_view p view_t false)
+  (r: ref view_t p)
+: Steel view_t
+  (r `pts_to_view` vw)
+  (fun _ -> r `pts_to_view` vw)
+  (requires (fun _ -> True))
+  (ensures (fun h res h' ->
+    res == h (r `pts_to_view` vw) /\
+    res == h' (r `pts_to_view` vw)
+  ))
+
+val pts_to_view_or_null_hp
+  (#view_t: Type u#0)
+  (#view_t': Type u#0)
+  (#b: Type u#b) (#p: pcm b)
+  (r: ptr view_t p) (view: sel_view p view_t' false)
+: Tot (Steel.Memory.slprop u#1)
+
+val pts_to_view_or_null_sel
+  (#view_t: Type u#0)
+  (#view_t': Type u#0)
+  (#b: Type u#b) (#p: pcm b)
+  (r: ptr view_t p) (view: sel_view p view_t' false)
+: Tot (selector (option view_t') (pts_to_view_or_null_hp r view))
+
+[@@__steel_reduce__]
+let pts_to_view_or_null
+  (#view_t: Type u#0)
+  (#view_t': Type u#0)
+  (#b: Type u#b) (#p: pcm b)
+  (r: ptr view_t p) (view: sel_view p view_t' false)
+: vprop
+= VUnit ({
+    hp = pts_to_view_or_null_hp r view;
+    t = _;
+    sel = pts_to_view_or_null_sel r view;
+  })
+
+val intro_pts_to_view_or_null_null
+  (#inames: _)
+  (#b: Type) (#p: pcm b)
+  (#c: Type0)
+  (vw: sel_view p c false)
+: SteelGhost unit inames
+    emp
+    (fun _ -> pts_to_view_or_null (null c p) vw)
+    (requires (fun _ -> True))
+    (ensures (fun _ _ h' -> h' (pts_to_view_or_null (null c p) vw) == None))
+
+val elim_pts_to_view_or_null_null
+  (#inames: _)
+  (#b: Type) (#p: pcm b)
+  (#c: Type0)
+  (r: ptr c p)
+  (vw: sel_view p c false)
+: SteelGhost unit inames
+    (pts_to_view_or_null r vw)
+    (fun _ -> emp)
+    (requires (fun _ -> ptr_is_null r == true))
+    (ensures (fun _ _ _ -> True))
+
+val intro_pts_to_view_or_null_not_null
+  (#inames: _)
+  (#b: Type) (#p: pcm b)
+  (#c: Type0)
+  (r: ref c p)
+  (vw: sel_view p c false)
+: SteelGhost unit inames
+    (pts_to_view r vw)
+    (fun _ -> pts_to_view_or_null r vw)
+    (requires (fun _ -> True))
+    (ensures (fun h _ h' -> h' (pts_to_view_or_null r vw) == Some (h (pts_to_view r vw))))
+
+val elim_pts_to_view_or_null_not_null
+  (#inames: _)
+  (#b: Type) (#p: pcm b)
+  (#c: Type0)
+  (r: ref c p)
+  (vw: sel_view p c false)
+: SteelGhost unit inames
+    (pts_to_view_or_null r vw)
+    (fun _ -> pts_to_view r vw)
+    (requires (fun _ -> True))
+    (ensures (fun h _ h' -> h (pts_to_view_or_null r vw) == Some (h' (pts_to_view r vw))))
+
+val freeable
+  (#view_t: Type u#0) (#b: Type u#0) (#q: pcm b)
+  (r: ref view_t q)
+: Tot prop
+
+(* Operations on views *)
+
+let refine_view
+  (#carrier: Type u#a)
+  (#p: pcm carrier)
+  (#view: Type u#b)
+  (#can_view_unit:bool)
+  (vw: sel_view p view can_view_unit)
+  (pr: (view -> Tot prop))
+: Tot (sel_view p (refine view pr) can_view_unit)
+= {
+  to_view_prop = (fun (c: carrier) -> vw.to_view_prop c /\ pr (vw.to_view c));
+  to_view = (fun c -> vw.to_view c <: refine view pr);
+  to_carrier = (fun (v: refine view pr) -> vw.to_carrier v <: carrier);
+  to_carrier_not_one = vw.to_carrier_not_one;
+  to_view_frame = (fun x frame -> vw.to_view_frame x frame);
+}
+
+inline_for_extraction
+noextract
+val intro_refine_view
+  (#opened: _)
+  (#carrier: Type u#a)
+  (#p: pcm carrier)
+  (#view: Type)
+  (vw: sel_view p view false)
+  (pr: (view -> Tot prop))
+  (r: ref view p)
+: SteelAtomicBase (ref (refine view pr) p) false opened Unobservable
+    (pts_to_view r vw)
+    (fun r' -> pts_to_view r' (refine_view vw pr))
+    (fun h -> pr (h (pts_to_view r vw)))
+    (fun h r' h' ->
+      let x = h (pts_to_view r vw) in
+      pr x /\
+      x == h' (pts_to_view r' (refine_view vw pr))
+    )
+
+inline_for_extraction
+noextract
+val elim_refine_view
+  (#opened: _)
+  (#carrier: Type u#a)
+  (#p: pcm carrier)
+  (#view: Type)
+  (vw: sel_view p view false)
+  (pr: (view -> Tot prop))
+  (r: ref (refine view pr) p)
+: SteelAtomicBase (ref view p) false opened Unobservable
+    (pts_to_view r (refine_view vw pr))
+    (fun r' -> pts_to_view r' vw)
+    (fun h -> True)
+    (fun h r' h' ->
+      let x = h' (pts_to_view r' vw) in
+      pr x /\
+      x == h (pts_to_view r (refine_view vw pr))
+    )
+
+let rewrite_view
+  (#carrier: Type u#a)
+  (#p: pcm carrier)
+  (#view: Type u#b)
+  (#can_view_unit:bool)
+  (vw: sel_view p view can_view_unit)
+  (#view' : Type u#c)
+  (f: view -> view')
+  (g: view' -> view)
+  (prf: squash (f `Steel.C.Model.Connection.is_inverse_of` g))
+: Tot (sel_view p view' can_view_unit)
+= {
+  to_view_prop = vw.to_view_prop;
+  to_view = (fun c -> f (vw.to_view c));
+  to_carrier = (fun v -> vw.to_carrier (g v));
+  to_carrier_not_one = vw.to_carrier_not_one;
+  to_view_frame = (fun x frame -> vw.to_view_frame (g x) frame);
+}
+
+inline_for_extraction
+noextract
+val intro_rewrite_view
+  (#opened: _)
+  (#carrier: Type u#a)
+  (#p: pcm carrier)
+  (#view: Type)
+  (vw: sel_view p view false)
+  (#view' : Type)
+  (f: view -> view')
+  (g: view' -> view)
+  (prf: squash (f `Steel.C.Model.Connection.is_inverse_of` g))
+  (r: ref view p)
+  (x' : Ghost.erased view')
+: SteelAtomicBase (ref view' p) false opened Unobservable
+    (pts_to_view r vw)
+    (fun r' -> pts_to_view r' (rewrite_view vw f g prf))
+    (fun h -> h (pts_to_view r vw) == g x')
+    (fun h r' h' ->
+      f (h (pts_to_view r vw)) == Ghost.reveal x' /\
+      h' (pts_to_view r' (rewrite_view vw f g prf)) == Ghost.reveal x'
+    )
+
+inline_for_extraction
+noextract
+val elim_rewrite_view
+  (#opened: _)
+  (#carrier: Type u#a)
+  (#p: pcm carrier)
+  (#view: Type)
+  (vw: sel_view p view false)
+  (#view' : Type)
+  (f: view -> view')
+  (g: view' -> view)
+  (prf: squash (f `Steel.C.Model.Connection.is_inverse_of` g))
+  (r: ref view' p)
+: SteelAtomicBase (ref view p) false opened Unobservable
+    (pts_to_view r (rewrite_view vw f g prf))
+    (fun r' -> pts_to_view r' vw)
+    (fun _ -> True)
+    (fun h r' h' ->
+      let x = h (pts_to_view r (rewrite_view vw f g prf)) in
+      let x' = h' (pts_to_view r' vw) in
+      Ghost.reveal x' == g (Ghost.reveal x) /\
+      f (Ghost.reveal x') == Ghost.reveal x
+    )
